theories/Spilling/RegLive.v
@@ -1,0 +1,55 @@
+Require Import List Map Env AllInRel Exp MoreList.
+Require Import IL Annotation.
+Require Import Liveness.Liveness.
+Require Import ExpVarsBounded SpillSound OneOrEmpty.
+
+
+
+Set Implicit Arguments.
+
+(** * Register Liveness *)
+
+Fixpoint reg_live 
+         (Lv : list ⦃var⦄)
+         (ZL : list params)
+         (G : ⦃var⦄)
+         (s : stmt)
+         (sl : spilling)
+         {struct s}
+  : ann ⦃var⦄
+  :=
+    match s, sl with
+    | stmtLet x e s, ann1 (Sp, L, _) sl'
+      => let lv_s := reg_live Lv ZL (singleton x) s sl' in
+        (* subtracting L might lead to unnecessary gaps in the liveness, but this is ok:
+           variables are killed from the register directly after their last use *)
+        ann1 (G ∪ Sp ∪ (((getAnn lv_s) \ singleton x ∪ Exp.freeVars e) \ L)) lv_s
+
+    | stmtReturn e, ann0 (Sp, L, _)
+      => ann0 (G ∪ Sp ∪ (Op.freeVars e \ L))
+
+    | stmtIf e s1 s2, ann2 (Sp, L, _) sl1 sl2
+      => let lv1 := reg_live Lv ZL ∅ s1 sl1 in
+        let lv2 := reg_live Lv ZL ∅ s2 sl2 in
+        ann2 (G ∪ Sp ∪ ((getAnn lv1 ∪ getAnn lv2 ∪ Op.freeVars e) \ L)) lv1 lv2
+
+    | stmtApp f Y, ann0 (Sp, L, (_,Sl)::nil)
+      => let blv := nth (counted f) Lv ∅ in
+        let Z   := nth (counted f) ZL nil in
+        ann0 (G ∪ Sp ∪ (((list_union (Op.freeVars ⊝ Y) ∩ Sl) ∪ blv \ of_list Z) \ L))
+
+    | stmtFun F t, annF (Sp, L, rms) sl_F sl_t
+      => let lv_t := reg_live (fst ⊝ rms ++ Lv) (fst ⊝ F ++ ZL) ∅ t sl_t in
+        let lv_F := (fun ps sl_s => reg_live (fst ⊝ rms ++ Lv)
+                                          (fst ⊝ F   ++ ZL)
+                                          (of_list (fst ps))
+                                          (snd ps)
+                                           sl_s
+                    ) ⊜ F sl_F in
+        annF (G ∪ Sp ∪ ((getAnn lv_t ∪ G) \ L)) lv_F lv_t
+
+    | _,_ => ann0 G
+    end
+.
+
+                                               
