theories/Spilling/RepairSpillInv.v
@@ -1,0 +1,14 @@
+Require Import RepairSpill.
+Require Import SpillSound Annotation Liveness.Liveness.
+Require Import List Map IL.
+
+Set Implicit Arguments.
+
+(** * Invariance on correct spillings *)
+
+(* assumptions missing *)
+Lemma repair_spill_inv
+  : live_sound Imperative ZL (merge ⊝ Λ) s lv
+    -> spill_sound k ZL Λ (R,M) s sl
+    -> sl === repair_spill k ZL Λ R M s lv sl
+.
