theories/Spilling/RepairSpillSound.v
@@ -1,0 +1,16 @@
+Require Import RepairSpill RegLive.
+Require Import SpillSound Annotation Liveness.Liveness.
+Require Import List Map IL.
+
+Set Implicit Arguments.
+
+(** * Soundness of repair_spill *)
+
+(* assumptions missing*)
+(* rlv does NOT have to be the correct reg liveness! (maybe it should have the right structure) *)
+Lemma repair_spill_sound k ZL Λ R M s rlv lv sl
+  : live_sound Imperative ZL (merge ⊝ Λ) s lv
+    -> spill_sound k ZL Λ (R,M) s (repair_spill k ZL Λ R M s rlv lv sl)
+.
+  
+                
